#120 removed not required da property, renamed everything

untimed/CaseStudy/Automaton.thy
@@ -3,253 +3,161 @@
     e-mail:       sebastian.stueber@rwth-aachen.de
 
     Description:  Frontend for deterministic Automatons, transformed from MontiArc-Automaton
+    Abbreviation: "da" for deterministic automaton
 *)
 
-theory Automaton
+theory dAutomaton
+  imports "../SPF"  "../SpfStep"
 
-imports "../SPF" "../../inc/Event" "../SpfStep"
 begin
-default_sort type
 
-section \<open>Backend Signatures\<close>
-(* This stuff is only here until the functions are defined in the backend, they will be in SPF.thy *)
+  default_sort type
 
+(* VERY Basic automaton wellformed condition *)
+fun daWell::"((('state \<times>(channel \<rightharpoonup> 'm::message)) \<Rightarrow> ('state \<times> 'm SB)) \<times> 'state \<times> 'm SB \<times> channel set \<times> channel set) \<Rightarrow> bool " where
+"daWell (transition, initialState, initialOut, chIn, chOut) = (finite chIn (* \<and> (\<forall>s f. (dom f = chIn \<and> sbElemWell f) \<longrightarrow> ubDom\<cdot>(snd(transition (s,f))) = chOut)*))"
 
-(* VERY Basic automaton type *)
-(* ToDo: wellformed condition *)
-
-(* FYI: in the non-deterministic case the automaton will be a cpo *)
-
-(* The content is:
-  transition function \<times> initial state \<times> initial Output \<times> input domain \<times> output domain *)
-
-fun automaton_well::"((('state \<times>(channel \<rightharpoonup> 'm::message)) \<Rightarrow> ('state \<times> 'm SB)) \<times> 'state \<times> 'm SB \<times> channel set \<times> channel set) \<Rightarrow> bool " where
-"automaton_well (transition, initialState, initialOut, chIn, chOut) = (finite chIn \<and> (\<forall>s f. (dom f = chIn \<and> sbElemWell f) \<longrightarrow> ubDom\<cdot>(snd(transition (s,f))) = chOut))"
-
-lemma automaton_wellI: assumes "finite In" 
-                           and "\<And>s f. (dom f = In \<and> sbElemWell f) \<Longrightarrow> ubDom\<cdot>(snd(transition (s,f))) = Out" 
-                         shows "automaton_well (transition, initialState, initialOut, In, Out)"
+lemma dawellI: assumes "finite In" 
+                         (*   and "\<And>s f. (dom f = In \<and> sbElemWell f) \<Longrightarrow> ubDom\<cdot>(snd(transition (s,f))) = Out"  *)
+                         shows "daWell (transition, initialState, initialOut, In, Out)"
   by(simp add: assms)
 
 
-lemma automaton_ex:"automaton_well ((\<lambda>f. (myState, ubLeast {})), State, ubLeast {}, {}, {})"
-  by(rule automaton_wellI,auto)
+lemma automaton_ex:"daWell ((\<lambda>f. (myState, ubLeast {})), State, ubLeast {}, {}, {})"
+  by(rule dawellI,auto)
 
 
 
-typedef ('state::type, 'm::message) automaton =
-  "{f::(('state \<times>(channel \<rightharpoonup> 'm)) \<Rightarrow> ('state \<times> 'm SB)) \<times> 'state \<times> 'm SB \<times> channel set \<times> channel set. automaton_well f}"
-  using automaton_ex exI automaton_wellI  by fastforce
 
-setup_lifting type_definition_automaton
+(* The content is:
+  transition function \<times> initial state \<times> initial Output \<times> input domain \<times> output domain *)
+typedef ('state::type, 'm::message) dAutomaton =
+  "{f::(('state \<times>(channel \<rightharpoonup> 'm)) \<Rightarrow> ('state \<times> 'm SB)) \<times> 'state \<times> 'm SB \<times> channel set \<times> channel set. daWell f}"
+  by auto
 
-definition getTransition :: "('s, 'm::message) automaton \<Rightarrow> (('s \<times>(channel \<rightharpoonup> 'm)) \<Rightarrow> ('s \<times> 'm SB))" where
-"getTransition automat = fst (Rep_automaton automat)"
-
-definition getInitialState :: "('s, 'm::message) automaton \<Rightarrow> 's" where
-"getInitialState automat = fst (snd (Rep_automaton automat))"
-
-definition getInitialOutput :: "('s, 'm::message) automaton \<Rightarrow> 'm SB" where
-"getInitialOutput automat = fst (snd (snd (Rep_automaton automat)))"
-
-definition getDom :: "('s, 'm::message) automaton \<Rightarrow> channel set" where
-"getDom automat = fst (snd (snd (snd (Rep_automaton automat))))"
-
-definition getRan :: "('s, 'm::message) automaton \<Rightarrow> channel set" where
-"getRan automat = (snd (snd (snd (snd (Rep_automaton automat)))))"
+setup_lifting type_definition_dAutomaton
 
 
-definition helper:: "(('s \<times>'e) \<Rightarrow> ('s \<times> 'm::message  SB)) \<Rightarrow> 's \<Rightarrow> ('s \<Rightarrow> 'm SPF) \<rightarrow> ('e \<Rightarrow> 'm SPF)" where
-"helper f s \<equiv> \<Lambda> h. (\<lambda> e. spfRt\<cdot>(spfConc (snd (f (s,e)))\<cdot>(h (fst (f (s,e))))))"
 
-lemma helper_cont: "cont (\<lambda>h. (\<lambda> e. spfConc (snd (f (s,e)))\<cdot>(h (fst (f (s,e))))))"
-  by simp
+
+
+(*******************************************************************)
+  section \<open>Definitions\<close>
+(*******************************************************************)
+
+definition daTransition :: "('s, 'm::message) dAutomaton \<Rightarrow> (('s \<times>(channel \<rightharpoonup> 'm)) \<Rightarrow> ('s \<times> 'm SB))" where
+"daTransition automat = fst (Rep_dAutomaton automat)"
+
+definition daInitialState :: "('s, 'm::message) dAutomaton \<Rightarrow> 's" where
+"daInitialState automat = fst (snd (Rep_dAutomaton automat))"
+
+definition daInitialOutput :: "('s, 'm::message) dAutomaton \<Rightarrow> 'm SB" where
+"daInitialOutput automat = fst (snd (snd (Rep_dAutomaton automat)))"
+
+definition daDom :: "('s, 'm::message) dAutomaton \<Rightarrow> channel set" where
+"daDom automat = fst (snd (snd (snd (Rep_dAutomaton automat))))"
+
+definition daRan :: "('s, 'm::message) dAutomaton \<Rightarrow> channel set" where
+"daRan automat = (snd (snd (snd (snd (Rep_dAutomaton automat)))))"
+
+
+(* Given a state and an input it returns the next state *)
+definition daNextState:: "('s::type, 'm::message) dAutomaton \<Rightarrow> 's \<Rightarrow>  ((channel \<rightharpoonup> 'm)) \<Rightarrow> 's" where
+"daNextState aut s m = fst ((daTransition aut) (s,m))"
+
+(* Given a state and an input it returns the next output *)
+definition daNextOutput:: "('s::type, 'm::message) dAutomaton \<Rightarrow> 's \<Rightarrow>  ((channel \<rightharpoonup> 'm)) \<Rightarrow>  'm SB" where
+"daNextOutput aut s m = snd ((daTransition aut) (s,m))"
+
+
+
+
+definition da_helper:: "(('s \<times>'e) \<Rightarrow> ('s \<times> 'm::message  SB)) \<Rightarrow> 's \<Rightarrow> ('s \<Rightarrow> 'm SPF) \<rightarrow> ('e \<Rightarrow> 'm SPF)" where
+"da_helper f s \<equiv> \<Lambda> h. (\<lambda> e. spfRt\<cdot>(spfConc (snd (f (s,e)))\<cdot>(h (fst (f (s,e))))))"
 
 (* As defined in Rum96 *)
-definition h :: "('s::type, 'm::message) automaton \<Rightarrow> ('s \<Rightarrow> 'm SPF)" where
-"h automat = spfStateFix (getDom automat)(getRan automat)\<cdot>
-     (\<Lambda> h. (\<lambda>s. spfStep  (getDom automat) (getRan automat)\<cdot>(helper (getTransition automat) s\<cdot>h)))"
-
-lemma h_cont: "cont (\<lambda> h. (\<lambda>s. spfStep  (getDom automat) (getRan automat)\<cdot>(helper (getTransition automat) s\<cdot>h)))"
-  by simp
+definition da_h :: "('s::type, 'm::message) dAutomaton \<Rightarrow> ('s \<Rightarrow> 'm SPF)" where
+"da_h automat = spfStateFix (daDom automat)(daRan automat)\<cdot>
+     (\<Lambda> h. (\<lambda>s. spfStep  (daDom automat) (daRan automat)\<cdot>(da_helper (daTransition automat) s\<cdot>h)))"
 
 (* This function also prepends the first SB ... *)
 (* But basically she just calls h *)
-definition H :: "('s, 'm::message) automaton \<Rightarrow> 'm SPF" where
-"H automat = spfConc (getInitialOutput automat)\<cdot>(h automat (getInitialState automat))"
+definition da_H :: "('s, 'm::message) dAutomaton \<Rightarrow> 'm SPF" where
+"da_H automat = spfConc (daInitialOutput automat)\<cdot>(da_h automat (daInitialState automat))"
 
 
-lemma automat_well[simp]:"automaton_well (Rep_automaton automat)"
-  using Rep_automaton by auto
 
-lemma automat_finite_dom[simp]:"finite (getDom automat)"
-  by (metis automat_well automaton_well.simps getDom_def surjective_pairing)
 
-    
-lemma ufLeast_apply:assumes "ubDom\<cdot>sb = In" shows "ufLeast In  Out \<rightleftharpoons> sb = ubclLeast Out"
-  apply (simp add: ufLeast_def)
-  unfolding ubclLeast_ubundle_def
-  unfolding ubclDom_ubundle_def
-  by (simp add: assms)
-    
-   
-lemma ubclDom2ubDom:"ubclDom\<cdot>sb = ubDom\<cdot>sb"
-  by (simp add: ubclDom_ubundle_def)
-    
-section \<open>Lemma about helper\<close>
+
+(*******************************************************************)
+  section \<open>Lemma\<close>
+(*******************************************************************)
+
+
+lemma da_rep_well[simp]:"daWell (Rep_dAutomaton automat)"
+  using Rep_dAutomaton by auto
+
+lemma da_dom_finite[simp]:"finite (daDom automat)"
+  by (metis da_rep_well daWell.simps daDom_def surjective_pairing)
+
+
+
+  section \<open>Lemma about helper\<close>
   
-lemma helper_dom:"ufDom\<cdot>((helper (getTransition automat) s\<cdot>(h automat)) f) = ufDom\<cdot>((h automat) s)"
-proof(simp add: helper_def)
-  show "ufDom\<cdot>(h automat (fst (getTransition automat (s, f)))) = ufDom\<cdot>((h automat) s)"
-    by(simp add: h_def spfstatefix_dom)
-qed
+lemma da_helper_dom [simp]:"ufDom\<cdot>((da_helper (daTransition automat) s\<cdot>(da_h automat)) f) = ufDom\<cdot>((da_h automat) s)"
+  by(simp add: da_helper_def da_h_def spfstatefix_dom)
+
+lemma da_helper_ran:"ufRan\<cdot>((da_helper (daTransition automat) s\<cdot>(da_h automat)) f) = ufRan\<cdot>((da_h automat) s)"
+  by(simp add: da_helper_def da_h_def spfstatefix_ran)
 
 
-lemma helper_ran:"ufRan\<cdot>((helper (getTransition automat) s\<cdot>(h automat)) f) = ufRan\<cdot>((h automat) s)"
-proof(simp add: helper_def)
-  show "ufRan\<cdot>(h automat (fst (getTransition automat (s, f)))) = ufRan\<cdot>(h automat s)"
-    by(simp add: h_def spfstatefix_ran)
-qed
 
-section \<open>Lemma about h\<close>
 
-lemma[simp]:"ufDom\<cdot>(h automat s) = getDom automat"
-  by(simp add: h_def spfstatefix_dom)
+  section \<open>Lemma about h\<close>
 
-lemma[simp]:"ufRan\<cdot>(h automat s) = getRan automat"
-  by(simp add: h_def spfstatefix_ran)
+lemma da_h_dom [simp]:"ufDom\<cdot>(da_h automat s) = daDom automat"
+  by(simp add: da_h_def spfstatefix_dom)
 
-(*Assumption for spfStep is always true for an automaton*)
-lemma automat_dom_ran_well[simp]:assumes "ubDom\<cdot>sb = getDom automat" 
-  shows "ufDom\<cdot>((helper (getTransition automat) s\<cdot>(h automat)) (spfStep_h2 (sbHdElem\<cdot>sb))) = getDom automat \<and>
-         ufRan\<cdot>((helper (getTransition automat) s\<cdot>(h automat)) (spfStep_h2 (sbHdElem\<cdot>sb))) = getRan automat"
-proof
-  show "ufDom\<cdot>((helper (getTransition automat) s\<cdot>(h automat)) (spfStep_h2 (sbHdElem\<cdot>sb))) = getDom automat"
-    by(simp add: helper_dom)
-next
-  show "ufRan\<cdot>((helper (getTransition automat) s\<cdot>(h automat)) (spfStep_h2 (sbHdElem\<cdot>sb))) = getRan automat"
-    by(simp add: helper_ran)
-qed
+lemma da_h_ran [simp]:"ufRan\<cdot>(da_h automat s) = daRan automat"
+  by(simp add: da_h_def spfstatefix_ran)
 
-lemma h_dom [simp]: "ufDom\<cdot>(h automat s) = getDom automat"
-  apply(simp add: h_def h_cont)
+lemma da_dom_ran_well[simp]:assumes "ubDom\<cdot>sb = daDom automat" 
+  shows "ufDom\<cdot>((da_helper (daTransition automat) s\<cdot>(da_h automat)) (spfStep_h2 (sbHdElem\<cdot>sb))) = daDom automat \<and>
+         ufRan\<cdot>((da_helper (daTransition automat) s\<cdot>(da_h automat)) (spfStep_h2 (sbHdElem\<cdot>sb))) = daRan automat"
+  apply rule
+   apply simp
+  by(simp add: da_helper_ran)
+
+
+lemma da_h_unfolding: "(da_h automat s) = spfStep (daDom automat) (daRan automat)\<cdot>(da_helper (daTransition automat) s\<cdot>(da_h automat))"
+  apply(simp add: da_h_def)
   by(subst spfStateFix_fix,simp_all)
 
-lemma h_ran [simp]: "ufRan\<cdot>(h automat s) = getRan automat"
-  apply(simp add: h_def h_cont)
-  by(subst spfStateFix_fix,simp_all)
- 
-lemma h_out_dom:assumes "ubDom\<cdot>sb = getDom automat" shows " ubDom\<cdot>(h automat state \<rightleftharpoons> sb) = getRan automat"
-  by (simp add: assms spf_ubDom)
-
-lemma h_unfolding: "(h automat s) = spfStep (getDom automat) (getRan automat)\<cdot>(helper (getTransition automat) s\<cdot>(h automat))"
-  apply(simp add: h_def)
-  by(subst spfStateFix_fix,simp_all)
-
-lemma h_step: assumes "ubDom\<cdot>sb = getDom automat" and "\<forall>c\<in>getDom automat. sb  .  c \<noteq> \<epsilon>"
-            shows "(h automat s)\<rightleftharpoons>sb = ((helper (getTransition automat) s\<cdot>(h automat)) ((inv convDiscrUp)(sbHdElem\<cdot>sb))) \<rightleftharpoons>sb"
-  apply (simp add: h_unfolding)
+lemma da_h_step: assumes "ubDom\<cdot>sb = daDom automat" and "\<forall>c\<in>daDom automat. sb  .  c \<noteq> \<epsilon>"
+            shows "(da_h automat s)\<rightleftharpoons>sb = ((da_helper (daTransition automat) s\<cdot>(da_h automat)) ((inv convDiscrUp)(sbHdElem\<cdot>sb))) \<rightleftharpoons>sb"
+  apply (simp add: da_h_unfolding)
   apply(rule SpfStep.stepstep_step)
   by (simp_all add: assms)
 
-definition autGetNextState:: "('s::type, 'm::message) automaton \<Rightarrow> 's \<Rightarrow>  ((channel \<rightharpoonup> 'm)) \<Rightarrow> 's" where
-"autGetNextState aut s m = fst ((getTransition aut) (s,m))"
-
-definition autGetNextOutput:: "('s::type, 'm::message) automaton \<Rightarrow> 's \<Rightarrow>  ((channel \<rightharpoonup> 'm)) \<Rightarrow>  'm SB" where
-"autGetNextOutput aut s m = snd ((getTransition aut) (s,m))"
-
-
 (* ToDo: make a bit more readable *)
-lemma h_final:
-  assumes "ubDom\<cdot>sb = getDom automat" and "\<forall>c\<in>getDom automat. sb  .  c \<noteq> \<epsilon>"
-  shows "(h automat s)\<rightleftharpoons>sb =
-  spfConc (autGetNextOutput automat s ((inv convDiscrUp)(sbHdElem\<cdot>sb)))\<cdot>(spfRt\<cdot>(h automat (autGetNextState automat s ((inv convDiscrUp)(sbHdElem\<cdot>sb))))) \<rightleftharpoons>sb"
-  apply(subst h_step, simp_all add: assms)
-  by (simp add: assms(1) autGetNextOutput_def autGetNextState_def helper_def spfRt_spfConc)
+lemma da_h_final:
+  assumes "ubDom\<cdot>sb = daDom automat" 
+      and "\<forall>c\<in>daDom automat. sb  .  c \<noteq> \<epsilon>"
+  shows "(da_h automat s)\<rightleftharpoons>sb =
+  spfConc (daNextOutput automat s ((inv convDiscrUp)(sbHdElem\<cdot>sb)))\<cdot>(spfRt\<cdot>(da_h automat (daNextState automat s ((inv convDiscrUp)(sbHdElem\<cdot>sb))))) \<rightleftharpoons>sb"
+  apply(subst da_h_step, simp_all add: assms)
+  by (simp add: assms(1) daNextOutput_def daNextState_def da_helper_def spfRt_spfConc)
     
-lemma h_bottom: assumes "ubDom\<cdot>sb = getDom automat" and "\<exists>c\<in>getDom automat. sb  .  c = \<epsilon>"
-  shows "(h automat s)\<rightleftharpoons>sb = ubclLeast (getRan automat)"
-  apply(simp add: h_unfolding spfStep_def, subst beta_cfun, subst spfStep_cont, simp_all add: spfStep_h1_def)
-  using assms(1) assms(2) sbHdElem_bottom_exI ufLeast_apply by blast
-
-section \<open>Lemma about H\<close>
+lemma da_h_bottom: assumes "ubDom\<cdot>sb = daDom automat" and "\<exists>c\<in>daDom automat. sb  .  c = \<epsilon>"
+  shows "(da_h automat s)\<rightleftharpoons>sb = ubclLeast (daRan automat)"
+  apply(simp add: da_h_unfolding spfStep_def, subst beta_cfun, subst spfStep_cont, simp_all add: spfStep_h1_def)
+  using assms(1) assms(2) sbHdElem_bottom_exI by (metis ubclDom_ubundle_def ufleast_apply) 
 
 
 
 
+  section \<open>Lemma about H\<close>
 
 
-
-
-(* From here everything should be automatically transformed from MontiArc-Automaton *)
-section \<open>Automaton Datatypes\<close>
-
-(* Only on idea how the states could be implemented *)
-datatype substate = even | odd  (* This are the actual states from MAA *)
-datatype myState = State substate nat bool (* And these have also the variables *)
-
-fun getVarI :: "myState \<Rightarrow> nat" where
-"getVarI (State _ n _) = n"
-
-fun getSubState :: "myState \<Rightarrow> substate" where
-"getSubState (State s _ _) = s"
-
-
-
-datatype myM = N nat | B bool
-
-instance myM :: countable
-apply(intro_classes)
-by(countable_datatype)
-
-
-instantiation myM :: message
-begin
-  fun ctype_myM :: "channel \<Rightarrow> myM set" where
-  "ctype_myM c1 = range N"  |
-  "ctype_myM c2 = range B"
-
-  instance
-    by(intro_classes)
-end
-
-
-
-section \<open>Automaton Functions\<close>
-
-(* Creates a fitting SB given the right output values *)
-(* Parameter:
-  nat         \<Rightarrow> maps to channel c1, in MAA called "XXXX"
-  bool        \<Rightarrow> maps to channel c2, in MAA calles "YYYY" *)
-lift_definition createOutput :: "nat \<Rightarrow> bool \<Rightarrow> myM SB" is
-"\<lambda>n b. ([c1 \<mapsto> \<up>(N n), c2 \<mapsto> \<up>(B b)])"
-  apply(auto simp add: ubWell_def)
-  sorry (* fails because stream instantiation is not there *)
-
-function test4 :: "(channel \<rightharpoonup> nat stream) \<Rightarrow> bool" where
-  "test4 [c1 \<mapsto> a] = True" |
-  "dom f \<noteq> {c1} \<Longrightarrow> test4 f = False"
-  sorry
-
-(* Somehow define the transition function *)
-(* use the createOutput function *)
-function myTransition :: "(myState \<times>(channel \<rightharpoonup> myM)) \<Rightarrow> (myState \<times> myM SB)" where
-"myTransition (State even n b,  [c1 \<mapsto> z])= (case z of N n \<Rightarrow> ((State odd n b), createOutput n True) | _ \<Rightarrow> undefined)" |
-"myTransition (State odd n b, [c1 \<mapsto> z]) = ((State even n b), createOutput 0 False)"  |
-
-"dom f\<noteq> {c1} \<Longrightarrow> myTransition (_,f) = undefined"
-  apply auto
-  apply (smt dom_eq_singleton_conv getSubState.elims myM.exhaust substate.exhaust)
-  using map_upd_eqD1 apply fastforce
-  apply (metis option.simps(3))
-  by (metis option.simps(3))
-
-lift_definition myAutomaton :: "(myState, myM) automaton" is "(myTransition, State even 0 True, ubLeast {}, {}, {})"
-  sorry  (* In the final form of the automaton datatype we will have to proof stuff *)
-
-definition mySPF :: "myM SPF" where
-"mySPF = H myAutomaton"
-
-section \<open>Automaton Lemma\<close>
 
 end
